1) fixed the definition of extractvalue and insertvalue, which can only use constant indices, unlike GEP that can use variable indices. LLVM expects that users store aggregate data into memory and access them via GEP, and aggregate data in registers are only used for multiple return values.
2) made 'const' type-annotated, these type information are useful when
translating constants into memory bytes where we need to consider target
layout wrt types. In LLVM, only at the cases where we cannot infer
types, constants are annotated with types. Types are omitted when such
types can be inferred, such as id = add i32 1, 2. We simply added
annotations at any case.

3) lowered GenericValue into list of memory bytes, and updated
semantics.



git-svn-id: https://webdav.seas.upenn.edu/svn/sol/vol@2483 eef5ea85-cc2e-0410-bd84-0fae1f012da8

src/ssa/llvm_op/ssa_interpreter.v
@@ -169,8 +169,8 @@ Definition switchToNewBasicBlock (Dest:block) (PrevBB:block) (Values:Mem): (bloc
 Definition getOperandValue (v:value) (Values:Mem) : option GenericValue := 
 match v with
 | value_id id => Values id
-| value_const (const_int n) => Some (GenericValue_int n)
-| value_const const_undef => Some (GenericValue_int 0)
+| value_const (const_int _ n) => Some (GenericValue_int n)
+| value_const (const_undef _) => Some (GenericValue_int 0)
 | _ => None
 end.
 
@@ -632,10 +632,10 @@ Inductive visitInst : State -> State -> trace -> Prop :=
       )::ECS)
     )
     trace_nil 
-| visitAddInsnt : forall CurSystem CurModule CurFunction CurBB Values VarArgs Caller ExitValue id t v1 v2 ECS i1 i2 CurInst',
+| visitAddInsnt : forall CurSystem CurModule CurFunction CurBB Values VarArgs Caller ExitValue id sz v1 v2 ECS i1 i2 CurInst',
   getOperandValue v1 Values = Some (GenericValue_int i1) ->
   getOperandValue v2 Values = Some (GenericValue_int i2) ->
-  getNextInsnFrom (insn_add id t v1 v2) CurBB = Some CurInst' ->
+  getNextInsnFrom (insn_add id sz v1 v2) CurBB = Some CurInst' ->
   visitInst 
     (mkState
       CurSystem
@@ -644,7 +644,7 @@ Inductive visitInst : State -> State -> trace -> Prop :=
       ((mkExecutionContext 
           CurFunction 
           CurBB 
-          (insn_add id t v1 v2) 
+          (insn_add id sz v1 v2) 
           Values 
           VarArgs 
           Caller
