src/ssa/opsem_conv.v
@@ -209,27 +209,27 @@ Definition dbInsn__implies__dsop_plus_prop state state' tr (db:dbInsn state stat
   dsop_plus state state' tr.
 Definition dbop__implies__dsop_star_prop state state' tr (db:dbop state state' tr) := 
   dsop_star state state' tr.
-Definition dbFdef__implies__dsop_star_prop fid rt lp S M ECs lc gl Mem lc' gl' als' Mem' B'' Result tr 
-           (db:dbFdef fid rt lp S M ECs lc gl Mem lc' gl' als' Mem' B'' Result tr) := 
+Definition dbFdef__implies__dsop_star_prop fid rt lp S TD Ps ECs lc gl Mem lc' gl' als' Mem' B'' Result tr 
+           (db:dbFdef fid rt lp S TD Ps ECs lc gl Mem lc' gl' als' Mem' B'' Result tr) := 
   forall B' I' la lb,
   lookupFdefViaIDFromSystemC S fid = Some (fdef_intro (fheader_intro rt fid la) lb) ->
   getEntryBlock (fdef_intro (fheader_intro rt fid la) lb) = Some B' ->
   getEntryInsn B' = Some I' ->
   dsop_star
-    (mkState S M ((mkEC (fdef_intro (fheader_intro rt fid la) lb) 
-                             B' I' (initLocals la (params2GVs lp lc gl))
-                            (params2GVs lp lc gl) nil)::ECs) gl Mem)
-    (mkState S M ((mkEC (fdef_intro (fheader_intro rt fid la) lb) 
+    (mkState S TD Ps ((mkEC (fdef_intro (fheader_intro rt fid la) lb) 
+                             B' I' (initLocals la (params2GVs TD lp lc gl))
+                            (params2GVs TD lp lc gl) nil)::ECs) gl Mem)
+    (mkState S TD Ps ((mkEC (fdef_intro (fheader_intro rt fid la) lb) 
                              B'' (insn_return rt Result) lc'
-                            (params2GVs lp lc gl) als')::ECs) gl' Mem')
+                            (params2GVs TD lp lc gl) als')::ECs) gl' Mem')
     tr
   .
 
 Lemma db__implies__ds:
   (forall state state' t  db, @dbInsn__implies__dsop_plus_prop state state' t db) /\
   (forall state state' t  db, @dbop__implies__dsop_star_prop state state' t db) /\
-  (forall fid rt lp S M ECs lc gl Mem lc' gl' als' Mem' B'' ret tr db, 
-     @dbFdef__implies__dsop_star_prop fid rt lp S M ECs lc gl Mem lc' gl' als' Mem' B'' ret tr db).
+  (forall fid rt lp S TD Ps ECs lc gl Mem lc' gl' als' Mem' B'' ret tr db, 
+     @dbFdef__implies__dsop_star_prop fid rt lp S TD Ps ECs lc gl Mem lc' gl' als' Mem' B'' ret tr db).
 Proof.
 (db_mutind_cases
   apply db_mutind with
@@ -247,16 +247,16 @@ Proof.
     apply H with (B'0:=B'0)(I':=I'0) in H0; auto.
     rewrite <- nil_app_trace__eq__trace.
     apply dsop_plus_cons with 
-      (state2:=mkState S M ((mkEC (fdef_intro (fheader_intro rt fid la) lb)
-                               B'0 I'0 (initLocals la (params2GVs lp lc gl)) 
-                               (params2GVs lp lc gl) nil)::
+      (state2:=mkState S TD Ps ((mkEC (fdef_intro (fheader_intro rt fid la) lb)
+                               B'0 I'0 (initLocals la (params2GVs TD lp lc gl)) 
+                               (params2GVs TD lp lc gl) nil)::
                         (mkEC F B (insn_call rid rt fid lp) lc arg als)::EC) 
                         gl Mem); auto.
     rewrite <- trace_app_nil__eq__trace.
     apply dsop_star_trans with 
-      (state2:=mkState S M ((mkEC (fdef_intro (fheader_intro rt fid la) lb) 
+      (state2:=mkState S TD Ps ((mkEC (fdef_intro (fheader_intro rt fid la) lb) 
                                B' (insn_return rt Result) lc'
-                               (params2GVs lp lc gl) als')::
+                               (params2GVs TD lp lc gl) als')::
                         (mkEC F B (insn_call rid rt fid lp) lc arg als)::EC) 
                         gl' Mem'); auto.
       apply dsInsn__implies__dsop_star.
@@ -294,22 +294,22 @@ Proof.
   destruct db__implies__ds as [_ [J _]]. eauto.
 Qed.
 
-Lemma dbFdef__implies__dsop_star : forall fid rt lp S M ECs lc gl Mem lc' gl' als' Mem' B'' Result tr B' I' la lb,
-  dbFdef fid rt lp S M ECs lc gl Mem lc' gl' als' Mem' B'' Result tr ->
+Lemma dbFdef__implies__dsop_star : forall fid rt lp S TD Ps ECs lc gl Mem lc' gl' als' Mem' B'' Result tr B' I' la lb,
+  dbFdef fid rt lp S TD Ps ECs lc gl Mem lc' gl' als' Mem' B'' Result tr ->
   lookupFdefViaIDFromSystemC S fid = Some (fdef_intro (fheader_intro rt fid la) lb) ->
   getEntryBlock (fdef_intro (fheader_intro rt fid la) lb) = Some B' ->
   getEntryInsn B' = Some I' ->
   dsop_star 
-    (mkState S M ((mkEC (fdef_intro (fheader_intro rt fid la) lb) 
-                             B' I' (initLocals la (params2GVs lp lc gl))
-                            (params2GVs lp lc gl) nil)::ECs) gl Mem)
-    (mkState S M ((mkEC (fdef_intro (fheader_intro rt fid la) lb) 
+    (mkState S TD Ps ((mkEC (fdef_intro (fheader_intro rt fid la) lb) 
+                             B' I' (initLocals la (params2GVs TD lp lc gl))
+                            (params2GVs TD lp lc gl) nil)::ECs) gl Mem)
+    (mkState S TD Ps ((mkEC (fdef_intro (fheader_intro rt fid la) lb) 
                              B'' (insn_return rt Result) lc'
-                            (params2GVs lp lc gl) als')::ECs) gl' Mem')
+                            (params2GVs TD lp lc gl) als')::ECs) gl' Mem')
     tr.
 Proof.
-  intros fid rt lp S M EC lc gl Mem lc' gl' als' Mem' B'' Result tr B' I' la lb H.
-  revert fid rt lp S M EC lc gl Mem lc' gl' als' Mem' B'' Result tr H B' I' la lb.
+  intros fid rt lp S TD Ps EC lc gl Mem lc' gl' als' Mem' B'' Result tr B' I' la lb H.
+  revert fid rt lp S TD Ps EC lc gl Mem lc' gl' als' Mem' B'' Result tr H B' I' la lb.
   destruct db__implies__ds as [_ [_ J]]. eauto.
 Qed.
 
@@ -341,15 +341,15 @@ Qed.
 (** First,we prove that dbInsn, dbop and dbFdef imply small-step semantics,
     by nested coinduction. *)
 
-Lemma dbFdefInf__implies__dsop_diverges : forall fid rt lp S M ECs lc gl Mem tr B' I' la lb,
-  dbFdefInf fid rt lp S M ECs lc gl Mem tr ->
+Lemma dbFdefInf__implies__dsop_diverges : forall fid rt lp S TD Ps ECs lc gl Mem tr B' I' la lb,
+  dbFdefInf fid rt lp S TD Ps ECs lc gl Mem tr ->
   lookupFdefViaIDFromSystemC S fid = Some (fdef_intro (fheader_intro rt fid la) lb) ->
   getEntryBlock (fdef_intro (fheader_intro rt fid la) lb) = Some B' ->
   getEntryInsn B' = Some I' ->
   dsop_diverges 
-    (mkState S M ((mkEC (fdef_intro (fheader_intro rt fid la) lb) B' I' 
-                        (initLocals la (params2GVs lp lc gl)) 
-                        (params2GVs lp lc gl) nil)::ECs) gl Mem)
+    (mkState S TD Ps ((mkEC (fdef_intro (fheader_intro rt fid la) lb) B' I' 
+                        (initLocals la (params2GVs TD lp lc gl)) 
+                        (params2GVs TD lp lc gl) nil)::ECs) gl Mem)
     tr.
 Proof.
   cofix CIH_dbFdefInf.
@@ -365,9 +365,9 @@ Proof.
     assert (HdbFdefInf:=H).
     inversion H; subst.
     apply dsop_diverges_intro with 
-      (state2:=mkState S M ((mkEC (fdef_intro (fheader_intro rt fid la) lb)
-                               B' I' (initLocals la (params2GVs lp lc gl)) 
-                               (params2GVs lp lc gl) nil)::
+      (state2:=mkState S TD Ps ((mkEC (fdef_intro (fheader_intro rt fid la) lb)
+                               B' I' (initLocals la (params2GVs TD lp lc gl)) 
+                               (params2GVs TD lp lc gl) nil)::
                         (mkEC F B (insn_call rid rt fid lp) lc arg als)::EC) 
                         gl Mem); 
       try solve [clear CIH_dbFdefInf CIH_dbInsnInf; auto].
@@ -388,7 +388,7 @@ Proof.
         apply CIH_dbopInf in H0. clear CIH_dbopInf.
         apply dsop_diverges_intro with (state2:=state2); auto.
 
-  intros fid rt lp S M ECs lc gl Mem tr B' I' la lb 
+  intros fid rt lp S TD Ps ECs lc gl Mem tr B' I' la lb 
     HdbFdefInf Hlookup HgetEntryBlock HgetEntryInsn.
   inversion HdbFdefInf; subst.
   rewrite Hlookup in H. inversion H; subst.
@@ -409,9 +409,9 @@ Proof.
   assert (HdbFdefInf:=H).
   inversion H; subst.
   apply dsop_diverges_intro with 
-    (state2:=mkState S M ((mkEC (fdef_intro (fheader_intro rt fid la) lb)
-                             B' I' (initLocals la (params2GVs lp lc gl)) 
-                             (params2GVs lp lc gl) nil)::
+    (state2:=mkState S TD Ps ((mkEC (fdef_intro (fheader_intro rt fid la) lb)
+                             B' I' (initLocals la (params2GVs TD lp lc gl)) 
+                             (params2GVs TD lp lc gl) nil)::
                       (mkEC F B (insn_call rid rt fid lp) lc arg als)::EC) 
                       gl Mem); 
     try solve [clear CIH_dbInsnInf; auto].
@@ -456,24 +456,24 @@ Definition nbInsn__implies__nsop_plus_prop state_tr states' (nb:nbInsn state_tr 
   nsop_plus (state_tr::nil) states'.
 Definition nbop_star__implies__nsop_star_prop states states' (nb:nbop_star states states') := 
   nsop_star states states'.
-Definition nbFdef__implies__nsop_star_prop fid rt lp S M ECs lc gl Mem tr lc_gl_als_Mem_block_re_trs 
-           (nb:nbFdef fid rt lp S M ECs lc gl Mem tr lc_gl_als_Mem_block_re_trs) := 
+Definition nbFdef__implies__nsop_star_prop fid rt lp S TD Ps ECs lc gl Mem tr lc_gl_als_Mem_block_re_trs 
+           (nb:nbFdef fid rt lp S TD Ps ECs lc gl Mem tr lc_gl_als_Mem_block_re_trs) := 
   forall B' I' la lb,
   lookupFdefViaIDFromSystemC S fid = Some (fdef_intro (fheader_intro rt fid la) lb) ->
   getEntryBlock (fdef_intro (fheader_intro rt fid la) lb) = Some B' ->
   getEntryInsn B' = Some I' ->
   nsop_star
-    ((mkState S M ((mkEC (fdef_intro (fheader_intro rt fid la) lb) 
-                             B' I' (initLocals la (params2GVs lp lc gl))
-                            (params2GVs lp lc gl) nil)::ECs) gl Mem, tr)::nil)
-    (returnStatesFromOp S M ECs lp lc gl rt fid la lb lc_gl_als_Mem_block_re_trs)
+    ((mkState S TD Ps ((mkEC (fdef_intro (fheader_intro rt fid la) lb) 
+                             B' I' (initLocals la (params2GVs TD lp lc gl))
+                            (params2GVs TD lp lc gl) nil)::ECs) gl Mem, tr)::nil)
+    (returnStatesFromOp S TD Ps ECs lp lc gl rt fid la lb lc_gl_als_Mem_block_re_trs)
   .
 
-Lemma returnStatesFromOp__nsop_star__updateStatesFromReturns : forall lc_gl_als_Mem_block_re_trs S M F B rid (rt:typ) (fid:id) lp (lc:GVMap) arg als EC I' lc gl rt fid la lb states,
+Lemma returnStatesFromOp__nsop_star__updateStatesFromReturns : forall lc_gl_als_Mem_block_re_trs S TD Ps F B rid (rt:typ) (fid:id) lp (lc:GVMap) arg als EC I' lc gl rt fid la lb states,
   getNextInsnFrom (insn_call rid rt fid lp) B = Some I' ->
-  updateStatesFromReturns S M F B I' lc rt arg als EC rid lc_gl_als_Mem_block_re_trs = Some states ->
+  updateStatesFromReturns S TD Ps F B I' lc rt arg als EC rid lc_gl_als_Mem_block_re_trs = Some states ->
   nsop_star
-    (returnStatesFromOp S M (mkEC F B (insn_call rid rt fid lp) lc arg als::EC)
+    (returnStatesFromOp S TD Ps (mkEC F B (insn_call rid rt fid lp) lc arg als::EC)
                         lp lc gl rt fid la lb lc_gl_als_Mem_block_re_trs)
     states.
 Proof.
@@ -491,11 +491,11 @@ Proof.
   Case "rt0_is_void".
     remember (free_allocas Mem' als') as Mem''.
     destruct Mem''; simpl in H0; try solve [inversion H0; subst].
-    remember (updateStatesFromReturns S M F B I' lc0 rt0 arg als EC rid lc_gl_als_Mem_block_re_trs) as states2.
+    remember (updateStatesFromReturns S TD Ps F B I' lc0 rt0 arg als EC rid lc_gl_als_Mem_block_re_trs) as states2.
     destruct states2; simpl in H0; inversion H0; subst.
     assert (
-      (mkState S M (mkEC F B I' lc0 arg als::EC) gl' m, tr)::s = 
-      ((mkState S M (mkEC F B I' lc0 arg als::EC) gl' m, tr)::nil) ++ s
+      (mkState S TD Ps (mkEC F B I' lc0 arg als::EC) gl' m, tr)::s = 
+      ((mkState S TD Ps (mkEC F B I' lc0 arg als::EC) gl' m, tr)::nil) ++ s
     ) as EQ. auto.
     rewrite EQ.
     apply nsop_star_cons; auto.
@@ -505,15 +505,15 @@ Proof.
       apply IHlc_gl_als_Mem_block_re_trs with (I':=I'); auto.
 
   Case "rt0_isnt_void".
-    remember (updateEnv lc0 gl' rid (getOperandValue re lc' gl')) as lc_gl.
+    remember (updateEnv lc0 gl' rid (getOperandValue TD re lc' gl')) as lc_gl.
     destruct lc_gl as [lc'' gl''].
     remember (free_allocas Mem' als') as Mem''.
     destruct Mem''; simpl in H0; try solve [inversion H0; subst].
-    remember (updateStatesFromReturns S M F B I' lc0 rt0 arg als EC rid lc_gl_als_Mem_block_re_trs) as states2.
+    remember (updateStatesFromReturns S TD Ps F B I' lc0 rt0 arg als EC rid lc_gl_als_Mem_block_re_trs) as states2.
     destruct states2; simpl in H0; inversion H0; subst.
     assert (
-      (mkState S M (mkEC F B I' lc'' arg als::EC) gl'' m, tr)::s = 
-      ((mkState S M (mkEC F B I' lc'' arg als::EC) gl'' m, tr)::nil) ++ s
+      (mkState S TD Ps (mkEC F B I' lc'' arg als::EC) gl'' m, tr)::s = 
+      ((mkState S TD Ps (mkEC F B I' lc'' arg als::EC) gl'' m, tr)::nil) ++ s
     ) as EQ. auto.
     rewrite EQ.
     apply nsop_star_cons; auto.
@@ -526,8 +526,8 @@ Qed.
 Lemma nb__implies__ns:
   (forall state_tr states' nb, @nbInsn__implies__nsop_plus_prop state_tr states' nb) /\
   (forall states states' nb, @nbop_star__implies__nsop_star_prop states states' nb) /\
-  (forall fid rt lp S M ECs lc gl Mem tr lc_gl_Mem_block_re_trs nb, 
-     @nbFdef__implies__nsop_star_prop fid rt lp S M ECs lc gl Mem tr lc_gl_Mem_block_re_trs nb).
+  (forall fid rt lp S TD Ps ECs lc gl Mem tr lc_gl_Mem_block_re_trs nb, 
+     @nbFdef__implies__nsop_star_prop fid rt lp S TD Ps ECs lc gl Mem tr lc_gl_Mem_block_re_trs nb).
 Proof.
 (nb_mutind_cases
   apply nb_mutind with
@@ -541,39 +541,39 @@ Proof.
   intros; subst; simpl; 
     try solve [
       intuition |
-      apply nsop_plus_trans with (states2:=(mkState S M (mkEC F B I' lc' arg als::EC) gl' Mem, tr)::nil); 
+      apply nsop_plus_trans with (states2:=(mkState S TD Ps (mkEC F B I' lc' arg als::EC) gl' Mem, tr)::nil); 
         try solve [auto | rewrite app_nil_end; eauto] |
       apply nsop_plus_trans with (states2:=(mkState S (module_intro TD Ps) (mkEC F B I' lc' arg als::EC) gl' Mem, tr)::nil); 
         try solve [auto | rewrite app_nil_end; eauto]
     ].
   Case "nbBranch_def".
-    apply nsop_plus_trans with (states2:=(mkState S M (mkEC F B' I' lc' arg als::EC) gl Mem, tr)::nil); auto.
+    apply nsop_plus_trans with (states2:=(mkState S TD Ps (mkEC F B' I' lc' arg als::EC) gl Mem, tr)::nil); auto.
       rewrite app_nil_end; eauto.
   Case "nbBranch_undef".
-    apply nsop_plus_trans with (states2:=(mkState S M (mkEC F B1' I1' lc1' arg als::EC) gl Mem, tr)::
-                                        (mkState S M (mkEC F B2' I2' lc2' arg als::EC) gl Mem, tr)::nil); auto.
+    apply nsop_plus_trans with (states2:=(mkState S TD Ps (mkEC F B1' I1' lc1' arg als::EC) gl Mem, tr)::
+                                        (mkState S TD Ps (mkEC F B2' I2' lc2' arg als::EC) gl Mem, tr)::nil); auto.
       rewrite app_nil_end; eauto.
   Case "nbBranch_uncond".
-    apply nsop_plus_trans with (states2:=(mkState S M (mkEC F B' I' lc' arg als::EC) gl Mem, tr)::nil); auto.
+    apply nsop_plus_trans with (states2:=(mkState S TD Ps (mkEC F B' I' lc' arg als::EC) gl Mem, tr)::nil); auto.
       rewrite app_nil_end; eauto.
   Case "nbCall".
     inversion n. subst.
     assert (Hlookup:=H0).
     apply H with (B':=B')(I':=I'0) in H0; auto.
     apply nsop_plus_trans with 
-      (states2:=(mkState S M ((mkEC (fdef_intro (fheader_intro rt fid la) lb)
-                               B' I'0 (initLocals la (params2GVs lp lc gl)) 
-                               (params2GVs lp lc gl) nil)::
+      (states2:=(mkState S TD Ps ((mkEC (fdef_intro (fheader_intro rt fid la) lb)
+                               B' I'0 (initLocals la (params2GVs TD lp lc gl)) 
+                               (params2GVs TD lp lc gl) nil)::
                               (mkEC F B (insn_call rid rt fid lp) lc arg als)::EC) 
                                gl Mem, tr)::nil); auto.
       rewrite app_nil_end; eauto.
 
       apply nsop_star_trans with 
-        (states2:=returnStatesFromOp S M (mkEC F B (insn_call rid rt fid lp) lc arg als::EC)
+        (states2:=returnStatesFromOp S TD Ps (mkEC F B (insn_call rid rt fid lp) lc arg als::EC)
                               lp lc gl rt fid la lb lc_gl_als_Mem_block_re_trs); auto.
       apply returnStatesFromOp__nsop_star__updateStatesFromReturns with (I':=I'); auto.
   Case "nbAlloca".
-    apply nsop_plus_trans with (states2:=(mkState S (module_intro TD Ps) (mkEC F B I' lc' arg (mb::als)::EC) gl' Mem', tr)::nil); auto.
+    apply nsop_plus_trans with (states2:=(mkState S TD Ps (mkEC F B I' lc' arg (mb::als)::EC) gl' Mem', tr)::nil); auto.
       rewrite app_nil_end; eauto.
 
   Case "nbop_star_cons".
@@ -629,20 +629,20 @@ Proof.
     apply nsop_plus_trans with (states2:=states2); auto.
 Qed.
 
-Lemma nbFdef__implies__nsop_star : forall fid rt lp S M ECs lc gl Mem tr lc_gl_als_Mem_block_re_trs B' I' la lb,
-  nbFdef fid rt lp S M ECs lc gl Mem tr lc_gl_als_Mem_block_re_trs ->
+Lemma nbFdef__implies__nsop_star : forall fid rt lp S TD Ps ECs lc gl Mem tr lc_gl_als_Mem_block_re_trs B' I' la lb,
+  nbFdef fid rt lp S TD Ps ECs lc gl Mem tr lc_gl_als_Mem_block_re_trs ->
   lookupFdefViaIDFromSystemC S fid = Some (fdef_intro (fheader_intro rt fid la) lb) ->
   getEntryBlock (fdef_intro (fheader_intro rt fid la) lb) = Some B' ->
   getEntryInsn B' = Some I' ->
   nsop_star
-    ((mkState S M ((mkEC (fdef_intro (fheader_intro rt fid la) lb) 
-                             B' I' (initLocals la (params2GVs lp lc gl))
-                            (params2GVs lp lc gl) nil)::ECs) gl Mem, tr)::nil)
-    (returnStatesFromOp S M ECs lp lc gl rt fid la lb lc_gl_als_Mem_block_re_trs)
+    ((mkState S TD Ps ((mkEC (fdef_intro (fheader_intro rt fid la) lb) 
+                             B' I' (initLocals la (params2GVs TD lp lc gl))
+                            (params2GVs TD lp lc gl) nil)::ECs) gl Mem, tr)::nil)
+    (returnStatesFromOp S TD Ps ECs lp lc gl rt fid la lb lc_gl_als_Mem_block_re_trs)
   .
 Proof.
-  intros fid rt lp S M ECs lc gl Mem tr lc_gl_als_Mem_block_re_trs B' I' la lb H.
-  revert fid rt lp S M ECs lc gl Mem tr lc_gl_als_Mem_block_re_trs H B' I' la lb.
+  intros fid rt lp S TD Ps ECs lc gl Mem tr lc_gl_als_Mem_block_re_trs B' I' la lb H.
+  revert fid rt lp S TD Ps ECs lc gl Mem tr lc_gl_als_Mem_block_re_trs H B' I' la lb.
   destruct nb__implies__ns as [_ [_ J]]. eauto.
 Qed.
 
@@ -674,15 +674,15 @@ Qed.
 (** First,we prove that nbInsn, nbop and nbFdef imply small-step semantics,
     by nested coinduction. *)
 
-Lemma nbFdefInf__implies__nsop_diverges : forall fid rt lp S M ECs lc gl Mem tr B' I' la lb trs',
-  nbFdefInf fid rt lp S M ECs lc gl Mem tr trs' ->
+Lemma nbFdefInf__implies__nsop_diverges : forall fid rt lp S TD Ps ECs lc gl Mem tr B' I' la lb trs',
+  nbFdefInf fid rt lp S TD Ps ECs lc gl Mem tr trs' ->
   lookupFdefViaIDFromSystemC S fid = Some (fdef_intro (fheader_intro rt fid la) lb) ->
   getEntryBlock (fdef_intro (fheader_intro rt fid la) lb) = Some B' ->
   getEntryInsn B' = Some I' ->
   nsop_diverges 
-    ((mkState S M ((mkEC (fdef_intro (fheader_intro rt fid la) lb) B' I' 
-                        (initLocals la (params2GVs lp lc gl)) 
-                        (params2GVs lp lc gl) nil)::ECs) gl Mem, tr)::nil) trs'.
+    ((mkState S TD Ps ((mkEC (fdef_intro (fheader_intro rt fid la) lb) B' I' 
+                        (initLocals la (params2GVs TD lp lc gl)) 
+                        (params2GVs TD lp lc gl) nil)::ECs) gl Mem, tr)::nil) trs'.
 Proof.
   cofix CIH_nbFdefInf.
 
@@ -696,15 +696,15 @@ Proof.
     assert (HnbFdefInf:=H).
     inversion H; subst.
     apply nsop_diverges_trans with 
-      (states':=(mkState S M ((mkEC (fdef_intro (fheader_intro rt fid la) lb)
-                               B' I' (initLocals la (params2GVs lp lc gl)) 
-                               (params2GVs lp lc gl) nil)::
+      (states':=(mkState S TD Ps ((mkEC (fdef_intro (fheader_intro rt fid la) lb)
+                               B' I' (initLocals la (params2GVs TD lp lc gl)) 
+                               (params2GVs TD lp lc gl) nil)::
                         (mkEC F B (insn_call rid rt fid lp) lc arg als)::EC) 
                         gl Mem, tr)::nil).
       apply nsop_plus_trans 
-        with (states2:=(mkState S M ((mkEC (fdef_intro (fheader_intro rt fid la) lb)
-                                         B' I' (initLocals la (params2GVs lp lc gl)) 
-                                         (params2GVs lp lc gl) nil)::
+        with (states2:=(mkState S TD Ps ((mkEC (fdef_intro (fheader_intro rt fid la) lb)
+                                         B' I' (initLocals la (params2GVs TD lp lc gl)) 
+                                         (params2GVs TD lp lc gl) nil)::
                                      (mkEC F B (insn_call rid rt fid lp) lc arg als)::EC) 
                                      gl Mem, tr)::nil); auto.
         rewrite app_nil_end; eauto.
@@ -724,7 +724,7 @@ Proof.
       apply CIH_nbopInf in H0.
       apply nsop_diverges_trans with (states':=states2); auto.
 
-  intros fid rt lp S M ECs lc gl Mem tr B' I' la lb trs 
+  intros fid rt lp S TD Ps ECs lc gl Mem tr B' I' la lb trs 
     HnbFdefInf Hlookup HgetEntryBlock HgetEntryInsn.
   inversion HnbFdefInf; subst.
   rewrite Hlookup in H. inversion H; subst.
@@ -745,15 +745,15 @@ Proof.
   assert (HnbFdefInf:=H).
   inversion H; subst.
   apply nsop_diverges_trans with 
-    (states':=(mkState S M ((mkEC (fdef_intro (fheader_intro rt fid la) lb)
-                             B' I' (initLocals la (params2GVs lp lc gl)) 
-                             (params2GVs lp lc gl) nil)::
+    (states':=(mkState S TD Ps ((mkEC (fdef_intro (fheader_intro rt fid la) lb)
+                             B' I' (initLocals la (params2GVs TD lp lc gl)) 
+                             (params2GVs TD lp lc gl) nil)::
                       (mkEC F B (insn_call rid rt fid lp) lc arg als)::EC) 
                       gl Mem, tr)::nil).
     apply nsop_plus_trans 
-      with (states2:=(mkState S M ((mkEC (fdef_intro (fheader_intro rt fid la) lb)
-                                       B' I' (initLocals la (params2GVs lp lc gl)) 
-                                       (params2GVs lp lc gl) nil)::
+      with (states2:=(mkState S TD Ps ((mkEC (fdef_intro (fheader_intro rt fid la) lb)
+                                       B' I' (initLocals la (params2GVs TD lp lc gl)) 
+                                       (params2GVs TD lp lc gl) nil)::
                                    (mkEC F B (insn_call rid rt fid lp) lc arg als)::EC) 
                                    gl Mem, tr)::nil); auto.
       rewrite app_nil_end; eauto.
